\documentclass{article}

\usepackage{amsmath}
\usepackage{amssymb}
\usepackage{amsfonts}
\usepackage{graphicx}
\usepackage{hyperref}
\hypersetup{
  colorlinks=true,
  linkcolor=blue, 
}

\newcommand{\1}{\mathbf{1}}
\newcommand{\E}{\mathbb{E}}
\newcommand{\R}{\mathbb{R}}
\newcommand{\Rcal}{\mathcal{R}}
\renewcommand{\P}{\mathbb{P}}
\renewcommand{\L}{\mathcal{L}}
\newcommand{\thetahat}{\hat\theta}
\newcommand{\ie}{\textit{i.e. }}
\newcommand{\var}{\operatorname{Var}}


\title{Advanced Deep Learning}
\author{Joris LIMONIER}
\begin{document}
\maketitle

\tableofcontents

\section{Proposed exercise lecture 02}
\paragraph{Prove equivalence of formulations for implicit and explicit methods.}
The implicit Euler method is given by:
\begin{equation}
  w^{k+1} = w^{k} - \tau \nabla \phi (w^{k+1})
\end{equation}
The explicit Euler method is given by:
\begin{equation}
  w^{k+1} = w^{k} - \tau \nabla \phi (w^{k})
\end{equation}

\section{Proposed exercise lecture 03}
\paragraph{Find a closed form for the exponential moving average.}
The recursive expression of the exponential moving average is given by:
\begin{equation}
  \begin{cases}
    \langle a \rangle_0^{\alpha} = (1 - \alpha) a_0                                              \\
    \langle a \rangle_{n+1}^{\alpha} = \alpha \langle a \rangle_n^\alpha +  (1 - \alpha) a_{n+1} \\
  \end{cases}
\end{equation}
\begin{align*}
           & \langle a \rangle_{n+1}^{\alpha} = \alpha \langle a \rangle_n^\alpha +  (1 - \alpha) a_{n+1}                                                                       \\
  \implies &
  \langle a \rangle_{n+1}^{\alpha} = \alpha \left[ \alpha \langle a \rangle_{n-1}^\alpha +  (1 - \alpha) a_{n} \right] +  (1 - \alpha) a_{n+1}                                  \\
  \implies &
  \langle a \rangle_{n+1}^{\alpha} = \alpha^2 \langle a \rangle_{n-1}^\alpha +  \alpha (1 - \alpha) a_{n} +  (1 - \alpha) a_{n+1}                                               \\
  \implies &
  \langle a \rangle_{n+1}^{\alpha} = \alpha^2 \left[ \alpha \langle a \rangle_{n-2}^\alpha +  (1 - \alpha) a_{n-1} \right] +  \alpha (1 - \alpha) a_{n} +  (1 - \alpha) a_{n+1} \\
  \implies &
  \langle a \rangle_{n+1}^{\alpha} = \alpha^3 \langle a \rangle_{n-2}^\alpha + \alpha^2 (1 - \alpha) a_{n-1} +  \alpha (1 - \alpha) a_{n} +  (1 - \alpha) a_{n+1}               \\
  \implies &
  \langle a \rangle_{n+1}^{\alpha} = \alpha^3 \langle a \rangle_{n-2}^\alpha + (1-\alpha) \sum_{k=0}^{2} \alpha^k a_{n+1 - k}                                                   \\
  \implies &
  \langle a \rangle_{n+1}^{\alpha} = \alpha^{n+1} \langle a \rangle_{0}^\alpha + (1-\alpha) \sum_{k=0}^{n} \alpha^k a_{n+1 - k}                                                   \\
  \implies &
  \langle a \rangle_{n+1}^{\alpha} = \alpha^{n+1} (1-\alpha)a_0 + (1-\alpha) \sum_{k=0}^{n} \alpha^k a_{n+1 - k}                                                   \\
  \implies &
  \langle a \rangle_{n+1}^{\alpha} = (1-\alpha) \sum_{k=0}^{n+1} \alpha^k a_{n+1 - k}                                                   \\
  \implies &
  \langle a \rangle_{n+1}^{\alpha} = (1-\alpha) \sum_{k=0}^{n+1} \alpha^{n+1-k} a_{k}                                                   \\
\end{align*}





\end{document}