\documentclass{article}

\usepackage{amsmath}
\usepackage{amssymb}
\usepackage{amsfonts}
\usepackage{graphicx}
\usepackage{hyperref}
\hypersetup{
  colorlinks=true,
  linkcolor=blue, 
}

\newcommand{\1}{\mathbf{1}}
\newcommand{\E}{\mathbb{E}}
\newcommand{\R}{\mathbb{R}}
\newcommand{\Rcal}{\mathcal{R}}
\renewcommand{\P}{\mathbb{P}}
\renewcommand{\L}{\mathcal{L}}
\newcommand{\thetahat}{\hat\theta}
\newcommand{\ie}{\textit{i.e. }}
\newcommand{\var}{\operatorname{Var}}


\title{Statistical learning theory}
\author{Joris LIMONIER}
\begin{document}
\maketitle

\tableofcontents

\section{Proposed exercise lecture 02}
\subsection{Home Exercise}
\paragraph{Demonstrate that the MAP (Maximum A Posteriori) classification rule is quadratic with respect to $x^*$.}

We have the following:
\begin{equation}
  \hat{y}^* = \arg \max_{k = 1, \ldots, k} \P \left( Y=k | X = x^* \right)
\end{equation}
We compute the probability:
\begin{align*}
  \arg \max_{k = 1, \ldots, k} \P \left( Y=k | X = x^* \right)
   & \underbrace{=}_{\text{Bayes}} \frac{\P(Y=k) \P(X=x^* | Y=k)}{\P(X=x^*)}        \\
   & \propto \P(Y=k) \P(X=x^* | Y=k)                                                \\
   & \propto \hat{\Pi}_k \mathcal{N}\left( x^*, \hat{\mu}_k, \hat{\Sigma}_k \right) \\
\end{align*}

\begin{align*}
  \hat{y}^*
   & = \arg \max_{k = 1, \ldots, k} \hat{\Pi}_k \mathcal{N}\left( x^*, \hat{\mu}_k, \hat{\Sigma}_k \right)                                                                                                                \\
   & = \arg \max_{k = 1, \ldots, k} \log \left[ \hat{\Pi}_k \right] + \log \left[\mathcal{N} \left( x^*, \hat{\mu}_k, \hat{\Sigma}_k \right) \right]                                                                      \\
   & = \arg \max_{k = 1, \ldots, k} \log \left[ \hat{\Pi}_k \right] + \log \left[\frac{1}{(2 \pi)^{N / 2}|\Sigma|^{1 / 2}} e^{-\frac{1}{2}(x^*-\mu)^{\top} \Sigma^{-1}(x^*-\mu)} \right]                                  \\
   & = \arg \max_{k = 1, \ldots, k} \underbrace{\log \left[ \hat{\Pi}_k \right]}_{\text{Constant w.r.t. } x^*} + \underbrace{\left[ -\frac{1}{2}(x^*-\mu)^{\top} \Sigma^{-1}(x^*-\mu) \right]}_{\text{Quadratic in } x^*} \\
   & - \underbrace{\log \left[(2 \pi)^{N / 2}|\Sigma|^{1 / 2} \right]}_{\text{Constant w.r.t. } x^*}                                                                                                                      \\
\end{align*}
The second term is Quadratic in $x^*$, the others are constant w.r.t. $x^*$, which completes the proof.

\section{Proposed exercise lecture 05}
\subsection{In-class Exercise}
\paragraph{Compute the derivative with respect to the means.}
\begin{align*}
  \nabla_{\mu_k}\mathcal{L}(\theta)
  & =
  \nabla_{\mu_k} \sum_{n=1}^N \log \left[ \sum_{k=1}^K \pi_k \mathcal{N}(x_n|\mu_k, \Sigma_k)\right]                   \\
   & =
  \sum_{n=1}^N \frac{\pi_k \mathcal{N}(x_n|\mu_k, \Sigma_k)}{\sum_{k=1}^K \pi_k \mathcal{N}(x_n|\mu_k, \Sigma_k)} \\
   & =
  \sum_{n=1}^N \frac{\pi_k \mathcal{N}(x_n|\mu_k, \Sigma_k)}{\sum_{k=1}^K \pi_k \mathcal{N}(x_n|\mu_k, \Sigma_k)} \Sigma^{-1} (x_n - \mu_k)\\
  %  & =
  % \sum_{n=1}^N \frac{\pi_k \mathcal{N}(x_n|\mu_k, \Sigma_k)}{\sum_{k=1}^K \pi_k \mathcal{N}(x_n|\mu_k, \Sigma_k)} \Sigma^{-1} (x_n - \mu_k)\\
\end{align*}

\section{Proposed exercise lecture 09}
\subsection{In-class Exercise}
Write the observed log-likelihood. \\
$X_1 \sim \mathcal{N}(\mu_1, \Sigma_{11})$ observed, $X_2 \sim \mathcal{N}(\mu_2, \Sigma_{22})$ missing.
\begin{align*}
  \L_{obs} (\theta, X)
  &= \int \L_{full} (\theta, X) dX^{mis} \\
  &= \int \P (X_1, X_2, \theta) dX_{2} \\
  &= \int \P(X_1, X_2, \theta) dX_{2} \\
  &= \int \P(X_1) \P(X_2 \mid X_1) dX_{2} \\
  &= \P(X_1) \int \P(X_2 \mid X_1) dX_{2} \\
  &= \prod_{i=1}^n \P(X_{i1}) \int \P(X_2 \mid X_1) dX_{2} \\
\end{align*}

\begin{align*}
  \log \P(X_{i1})
  &= \frac{n}{2}\log(\sigma_{11}^2) - \frac{1}{2} \sum_{i=1}^n \frac{(X_{i1} - \mu_1)^2}{\sigma_{11}^2} \\
  &= \frac{n}{2}\log(\sigma_{22} - \frac{\sigma_{21}^2}{\sigma_{11}}) - \frac{1}{2} \sum_{i=1}^n \frac{(X_{i2} - (\mu_2 + \frac{\sigma_{21}}{\sigma_{11}} (X_{i1} - \mu_1)))^2}{(\sigma_{22} - \frac{\sigma_{21}^2}{\sigma_{11}})^2} \\
\end{align*}



\end{document}